define valid in a decidable way

theories/acyclic.v
@@ -1,20 +1,19 @@
 From stdpp Require Import relations.
 From Coq Require Import ssreflect.
-From ambig Require Import grammar local_amb.
-(* TODO: reachable in a separate file *)
+From ambig Require Import grammar reachable.
 
 (* On the graph representation of the grammar: direct edge *)
 Inductive succ {Σ N : Type} (G : grammar Σ N) : relation N :=
   | succ_unary A B φ :
-    G ⊢ A ↦ unary B φ →
+    A ↦ unary B φ ∈ G →
     succ G A B
   | succ_left A B E φ :
-    G ⊢ A ↦ binary B E φ →
-    nullable G E = true →
+    A ↦ binary B E φ ∈ G →
+    nullable G E →
     succ G A B
   | succ_right A B E φ :
-    G ⊢ A ↦ binary E B φ →
-    nullable G E = true →
+    A ↦ binary E B φ ∈ G →
+    nullable G E →
     succ G A B
   .
 
@@ -29,27 +28,26 @@ Definition unit {Σ N : Type} (G : grammar Σ N) : Prop :=
 Definition acyclic {Σ N : Type} (G : grammar Σ N) : Prop :=
   ¬ ∃ A, ex_loop (succ G) A.
 
-Lemma acyclic_succ_flip_wf {Σ N} (G : grammar Σ N) :
+Fact acyclic_succ_flip_wf {Σ N} (G : grammar Σ N) :
   acyclic G → wf (flip (succ G)).
 Admitted.
 
 (* unit -> acyclic *)
 
-Definition loop {Σ N : Type} `{EqDecision N} (G : grammar Σ N) (A : N) (α : clause Σ N) : bool :=
-  match α with
-  | unary A' _ => bool_decide (A' = A)
-  | binary A1 A2 _ =>
-    (nullable G A2 && bool_decide (A1 = A)) ||
-    (nullable G A1 && bool_decide (A2 = A))
-  | _ => false
-  end.
-
 Definition deloop {Σ N : Type} `{EqDecision N} (G : grammar Σ N) : grammar Σ N := {|
   start := start G;
-  P A := filter (λ α, ¬ bool_decide (loop G A α)) (P G A)
+  ε_productions := ε_productions G;
+  atom_productions := atom_productions G;
+  unary_productions A B :=
+    if bool_decide (B = A) then None else unary_productions G A B;
+  binary_productions A Bl Br :=
+    if bool_decide ((nullable G Br ∧ Bl = A) ∨ (nullable G Bl ∧ Br = A))
+    then None else binary_productions G A Bl Br;
+  unary_predicate_axiom := unary_predicate_axiom G;
+  binary_predicate_axiom := binary_predicate_axiom G;
 |}.
 
-Lemma deloop_nullable {Σ N} `{EqDecision N} (G : grammar Σ N) A :
+Fact deloop_nullable {Σ N} `{EqDecision N} (G : grammar Σ N) A :
   nullable (deloop G) A = nullable G A.
 Admitted.
 
@@ -58,26 +56,32 @@ Lemma deloop_succ_irrefl {Σ N} `{EqDecision N} (G : grammar Σ N) :
 Proof.
   intros A HA.
   inversion HA; subst; clear HA.
-  - apply elem_of_list_filter in H. simpl in H. naive_solver.
-  - apply elem_of_list_filter in H. simpl in H.
-    rewrite deloop_nullable in H0. rewrite H0 in H.
-    naive_solver.
-  - apply elem_of_list_filter in H. simpl in H.
-    rewrite deloop_nullable in H0. rewrite H0 in H.
-    naive_solver.
+  - inversion H. by case_bool_decide.
+  - rewrite deloop_nullable in H0. inversion H.
+    case_bool_decide => //. naive_solver.
+  - rewrite deloop_nullable in H0. inversion H.
+    case_bool_decide => //. naive_solver.
+Qed.
+
+Lemma deloop_production_subset {Σ N} `{EqDecision N} (G : grammar Σ N) p :
+  p ∈ (deloop G) → p ∈ G.
+Proof.
+  intros Hp. destruct p as [A α]; destruct α => //.
+  all: inversion Hp; by case_bool_decide.
 Qed.
 
 Lemma deloop_succ_subrel {Σ N} `{EqDecision N} (G : grammar Σ N) :
   subrelation (succ (deloop G)) (succ G).
 Proof.
-  intros A B HAB.
-  destruct HAB; apply elem_of_list_filter in H; destruct H as [_ ?].
+  intros A B HAB. destruct HAB.
+  all: apply deloop_production_subset in H.
+  all: try rewrite deloop_nullable in H0.
   - eapply succ_unary; eauto.
-  - eapply succ_left; eauto. by rewrite -deloop_nullable.
-  - eapply succ_right; eauto. by rewrite -deloop_nullable.
+  - eapply succ_left; eauto.
+  - eapply succ_right; eauto.
 Qed.
 
-Lemma ex_loop_subrelation {A} (R1 R2 : relation A) x :
+Fact ex_loop_subrelation {A} (R1 R2 : relation A) x :
   subrelation R1 R2 →
   ex_loop R1 x → ex_loop R2 x.
 Admitted.
@@ -93,143 +97,140 @@ Proof.
   * eapply ex_loop_subrelation. apply deloop_succ_subrel. done.
 Qed.
 
-Lemma deloop_valid {Σ N} `{!EqDecision N} (G : grammar Σ N) t A w :
+Lemma deloop_valid {Σ N} `{!EqDecision N} (G : grammar Σ N) (t : tree Σ N) A w :
   t ▷ A ={deloop G}=> w →
   ✓{G} t.
 Proof.
-  intros [? [? Ht]].
   generalize dependent A.
   generalize dependent w.
-  induction Ht => w ? B ?.
-  all: apply elem_of_list_filter in H; destruct H as [_ ?].
-  - by constructor.
-  - by constructor.
-  - econstructor; eauto.
-  - econstructor; eauto.
+  induction t => w A [? [? Ht]].
+  - apply valid_ε_tree_inv in Ht.
+    apply deloop_production_subset in Ht.
+    by apply valid_ε_tree.
+  - apply valid_token_tree_inv in Ht.
+    apply deloop_production_subset in Ht.
+    by apply valid_token_tree.
+  - apply valid_unary_tree_inv in Ht as [φ [Hp [? ?]]].
+    apply deloop_production_subset in Hp.
+    eapply valid_unary_tree; eauto.
+    eapply IHt; by repeat split.
+  - apply valid_binary_tree_inv in Ht as [φ [Hp [? [? ?]]]].
+    apply deloop_production_subset in Hp.
+    eapply valid_binary_tree; eauto.
+    eapply IHt1; by repeat split.
+    eapply IHt2; by repeat split.
 Qed.
 
 Definition inf_amb_cond {Σ N : Type} `{EqDecision N} (G : grammar Σ N) (A : N) (w : sentence Σ) : Prop :=
   ∃ C w', reachable G A w C w' ∧ G ⊨ C ⇒ w' ∧
-    ((∃ φ, G ⊢ C ↦ unary C φ ∧ (w' ≠ [] → φ w')) ∨
-     (∃ E φ, G ⊢ C ↦ binary C E φ ∧ nullable G E = true) ∨
-     (∃ E φ, G ⊢ C ↦ binary E C φ ∧ nullable G E = true)).
+    ((∃ φ, C ↦ unary C φ ∈ G ∧ φ w') ∨
+     (∃ E φ, C ↦ binary C E φ ∈ G ∧ nullable G E) ∨
+     (∃ E φ, C ↦ binary E C φ ∈ G ∧ nullable G E)).
 
-Lemma sentence_amb_reachable {Σ N} (G : grammar Σ N) A w B w' :
-  reachable G A w B w' →
-  sentence_ambiguous G B w' →
-  sentence_ambiguous G A w.
-Admitted.
-
-Lemma strict_subtree_ne_unary {Σ N : Type} (t : tree Σ N) A :
-  t ≠ unary_tree A t.
+Lemma inf_amb_implies_derive_amb {Σ N} `{EqDecision N} (G : grammar Σ N) A w : 
+  inf_amb_cond G A w → derive_amb G A w.
 Proof.
-  induction t; naive_solver.
-Qed.
-
-Lemma strict_subtree_ne_binary_left {Σ N : Type} (t t' : tree Σ N) A :
-  t ≠ binary_tree A t t'.
-Proof.
-  induction t; naive_solver.
-Qed.
-
-Lemma strict_subtree_ne_binary_right {Σ N : Type} (t t' : tree Σ N) A :
-  t ≠ binary_tree A t' t.
-Proof.
-  induction t; naive_solver.
-Qed.
-
-Lemma inf_amb_implies_amb {Σ N} `{EqDecision N} (G : grammar Σ N) A w : 
-  inf_amb_cond G A w → sentence_ambiguous G A w.
-Proof.
-  move => [C [w' [Hr [[t [? [? ?]]] H]]]].
+  move => [C [w' [Hr [[t [Hrt [? ?]]] H]]]].
   destruct H as [[φ [? ?]] | [[E [φ [? HE]]] | [E [φ [? HE]]]]].
-  - eapply sentence_amb_reachable; first apply Hr.
-    exists t, (unary_tree C t). split => //.
-    split. repeat split => //. econstructor; naive_solver.
-    apply strict_subtree_ne_unary.
-  - eapply sentence_amb_reachable; first apply Hr.
-    apply nullable_spec in HE. destruct HE as [tε [? [? ?]]].
-    exists t, (binary_tree C t tε). split => //.
-    split. repeat split => /=. by rewrite H1 app_nil_r.
-    econstructor; naive_solver.
-    apply strict_subtree_ne_binary_left.
-  - eapply sentence_amb_reachable; first apply Hr.
-    apply nullable_spec in HE. destruct HE as [tε [? [? ?]]].
-    exists t, (binary_tree C tε t). split => //.
-    split. repeat split => /=. by rewrite H1 app_nil_l.
-    econstructor; naive_solver.
-    apply strict_subtree_ne_binary_right.
+  all: eapply reachable_derive_amb; first apply Hr.
+  - exists t, (unary_tree C t).
+    split; first done.
+    split; last apply strict_subtree_ne_unary. 
+    repeat split => //.
+    eapply valid_unary_tree; naive_solver.
+  - apply nullable_spec in HE as [tε [? [? ?]]].
+    exists t, (binary_tree C t tε).
+    split; first done.
+    split; last apply strict_subtree_ne_binary_left.
+    repeat split => //.
+    { simpl. have -> : tree_word tε = [] by done.
+      by rewrite app_nil_r. }
+    eapply valid_binary_tree; try naive_solver.
+    apply (binary_predicate_axiom G). naive_solver.
+  - apply nullable_spec in HE as [tε [? [? ?]]].
+    exists t, (binary_tree C tε t).
+    split; first done.
+    split; last apply strict_subtree_ne_binary_right.
+    repeat split => //.
+    { simpl. have -> : tree_word tε = [] by done.
+      by rewrite app_nil_l. }
+    eapply valid_binary_tree; try naive_solver.
+    apply (binary_predicate_axiom G). naive_solver.
 Qed.
 
-Global Instance valid_decidable Σ N (G : grammar Σ N) t : Decision (✓{G} t).
-Admitted.
-
-Lemma deloop_invalid {Σ N} `{!EqDecision N} (G : grammar Σ N) t A w :
+Lemma deloop_invalid {Σ N} `{!EqDecision N} (G : grammar Σ N) (t : tree Σ N) A w :
   t ▷ A ={G}=> w →
   ¬ ✓{deloop G} t →
   inf_amb_cond G A w.
 Proof.
-  move => [? [? H]] Hnot.
+  move => [? [? Ht]] Hnot.
   generalize dependent w.
   generalize dependent A.
-  induction t as [| B [a p] | B t IHt | B t1 IHt1 t2 IHt2 ] => A ? w ?.
-  all: inversion H; subst; clear H => /=.
-  - exfalso. apply Hnot. constructor.
-    eapply elem_of_list_filter. naive_solver.
-  - exfalso. apply Hnot. constructor.
-    eapply elem_of_list_filter. naive_solver.
-  - destruct (decide (✓{deloop G} t)).
-    + (* valid *)
-      have He : B = root t.
+  induction t as [| B [a p] | B t IHt | B t1 IHt1 t2 IHt2 ] => A HA w Hw.
+  all: simpl in HA; simpl in Hw; subst.
+  - apply valid_ε_tree_inv in Ht.
+    exfalso. by apply Hnot, valid_ε_tree.
+  - apply valid_token_tree_inv in Ht.
+    exfalso. by apply Hnot, valid_token_tree.
+  - apply valid_unary_tree_inv in Ht as [φ [? [? ?]]].
+    destruct (✓{deloop G} t) eqn:Heqn.
+    + (* valid *) clear IHt.
+      have He : root t = A.
       { eapply bool_decide_eq_true. apply not_false_iff_true. move => He.
-        apply Hnot. econstructor; eauto.
-        eapply elem_of_list_filter. apply bool_decide_eq_false in He.
-        naive_solver. }
-      exists (root t), (sentence_of t).
-      repeat split => //. rewrite He; constructor. by exists t; repeat split.
+        apply Hnot. simpl. rewrite He H.
+        apply Is_true_andb. naive_solver. }
+      exists (root t), (word t).
+      split; first by constructor; naive_solver.
+      split; first by exists t; repeat split.
       left. exists φ. naive_solver.
     + (* not valid *)
       edestruct IHt as [C [w' [? ?]]]; eauto.
       exists C, w'. split; last done.
-      econstructor; eauto.
-  - destruct (decide (✓{deloop G} t2)); first destruct (decide (✓{deloop G} t1)).
-    + (* both valid *)
-      have He : (nullable G (root t2) && bool_decide (root t1 = B)) ||
-      (nullable G (root t1) && bool_decide (root t2 = B)) = true.
-      { apply not_false_iff_true. move => He. apply Hnot.
-        econstructor; eauto.
-        eapply elem_of_list_filter. simpl. rewrite He. naive_solver. }
-      exists B, (sentence_of t1 ++ sentence_of t2).
-      repeat split => //. constructor. exists (binary_tree B t1 t2).
-      repeat split. econstructor; eauto.
-      right. destruct (orb_true_elim _ _ He) as [H|H].
-      all: destruct (andb_prop _ _ H) as [H1 H2].
-      all: apply bool_decide_eq_true in H2.
-      * left. exists (root t2), φ. naive_solver.
-      * right. exists (root t1), φ. naive_solver.
+      econstructor; naive_solver.
+  - apply valid_binary_tree_inv in Ht as [φ [? [? [? ?]]]].
+    destruct (✓{deloop G} t2) eqn:Heqn2; first destruct (✓{deloop G} t1) eqn:Heqn1.
+    + (* both valid *) clear IHt1 IHt2.
+      have He : (nullable G (root t2) ∧ root t1 = A) ∨
+        (nullable G (root t1) ∧ root t2 = A).
+      { eapply bool_decide_eq_true. apply not_false_iff_true. move => He.
+        apply Hnot. simpl. rewrite He H.
+        apply Is_true_andb. naive_solver. }
+      exists A, (word t1 ++ word t2). repeat split.
+      * constructor; naive_solver.
+      * exists (binary_tree A t1 t2). repeat split. eapply valid_binary_tree; eauto.
+      * right. destruct He as [[? ?] | [? ?]].
+        ** left. exists (root t2), φ. naive_solver.
+        ** right. exists (root t1), φ. naive_solver.
     + (* t1 not valid *)
       edestruct IHt1 as [C [w' [? ?]]]; eauto.
       exists C, w'. split; last done.
-      eapply reachable_left; eauto. by eexists; repeat split.
+      eapply reachable_left; eauto.
+      by eexists; repeat split.
     + (* t2 not valid *)
       edestruct IHt2 as [C [w' [? ?]]]; eauto.
       exists C, w'. split; last done.
-      eapply reachable_right; eauto. by eexists; repeat split.
+      eapply reachable_right; eauto.
+      by eexists; repeat split.
 Qed.
 
-Theorem deloop_amb {Σ N} `{EqDecision N} (G : grammar Σ N) A w :
-  sentence_ambiguous G A w ↔
-    sentence_ambiguous (deloop G) A w ∨ inf_amb_cond G A w.
+Theorem deloop_derive_amb {Σ N} `{EqDecision N} (G : grammar Σ N) A w :
+  derive_amb G A w ↔
+    derive_amb (deloop G) A w ∨ inf_amb_cond G A w.
 Proof.
   split.
   - intros [t1 [t2 [[? [? Ht1]] [[? [? Ht2]] Hne]]]].
-    destruct (decide (✓{deloop G} t2)); first destruct (decide (✓{deloop G} t1)).
-    + (* both valid *) left. exists t1, t2. by repeat split.
-    + (* t1 not valid *) right. eapply deloop_invalid; eauto. by repeat split.
-    + (* t2 not valid *) right. eapply deloop_invalid; eauto. by repeat split.
+    destruct (✓{deloop G} t2) eqn:Heqn2; first destruct (✓{deloop G} t1) eqn:Heqn1.
+    + (* both valid *) left.
+      exists t1, t2. repeat split; naive_solver.
+    + (* t1 not valid *) right.
+      apply (deloop_invalid G t1); first done.
+      by apply Is_true_false.
+    + (* t2 not valid *) right.
+      apply (deloop_invalid G t2); first done.
+      by apply Is_true_false.
   - intros [H|H].
     + destruct H as [t1 [t2 [[? [? Ht1]] [[? [? Ht2]] Hne]]]].
       exists t1, t2. repeat split => //.
-      all: by eapply deloop_valid; repeat split.
-    + by apply inf_amb_implies_amb.
+      all: by eapply deloop_valid.
+    + by apply inf_amb_implies_derive_amb.
 Qed.
