theories/grammar.v
@@ -1,13 +1,11 @@
-From stdpp Require Import relations.
+From stdpp Require Import relations list.
 From Coq Require Import ssreflect.
 
 (* sentence *)
 
-Definition position : Type := nat * nat.
-
 Record token (Σ : Type) := {
   letter : Σ;
-  pos : position;
+  pos : nat (* line number *) * nat (* column number *);
 }.
 
 Arguments letter {_}.
@@ -20,11 +18,31 @@ Notation "a @ p" := {|
 
 Definition sentence (Σ : Type) : Type := list (token Σ).
 
-Definition unary_predicate (Σ : Type) : Type := sentence Σ → Prop.
+(* predicate should be decidable *)
 
-Definition binary_predicate (Σ : Type) : Type := sentence Σ → sentence Σ → Prop.
+Definition unary_predicate (Σ : Type) : Type := sentence Σ → bool.
+Definition binary_predicate (Σ : Type) : Type := sentence Σ → sentence Σ → bool.
 
 (* grammar *)
+
+Record grammar (Σ N : Type) := {
+  start : N;
+  ε_productions : N → bool;
+  atom_productions : N → Σ → bool;
+  unary_productions : N → N → option (unary_predicate Σ);
+  binary_productions : N → N → N → option (binary_predicate Σ);
+  unary_predicate_axiom : ∀ φ : unary_predicate Σ, φ [];
+  binary_predicate_axiom : ∀ (φ : binary_predicate Σ) w1 w2,
+    (w1 = [] ∨ w2 = []) → φ w1 w2;
+}.
+
+Arguments start {_} {_}.
+Arguments ε_productions {_} {_}.
+Arguments atom_productions {_} {_}.
+Arguments unary_productions {_} {_}.
+Arguments binary_productions {_} {_}.
+Arguments unary_predicate_axiom {_} {_}.
+Arguments binary_predicate_axiom {_} {_}.
 
 Inductive clause (Σ N : Type) : Type :=
   | ε : clause Σ N
@@ -38,17 +56,45 @@ Arguments atom {_} {_}.
 Arguments unary {_} {_}.
 Arguments binary {_} {_}.
 
-Definition nonterm {Σ N : Type} (A : N) : clause Σ N := unary A (λ _, True).
+(* NOTE
 
-Record grammar (Σ N : Type) := {
-  start : N;
-  P : N → list (clause Σ N);
+One can also define the production set of a grammar as a function from N to list (clause Σ N).
+
+But this definition has two disadvantages:
+1. To show that (A ↦ α ∈ G) is decidable, we need to show that predicates are eq decidable, which is not so obvious (though in practice the predicates are taken from a predefined set)
+2. This definition fails to reject productions with conflicting predicates, e.g. A ↦ B offside and A ↦ B same_line.
+*)
+
+Inductive production (Σ N : Type) : Type :=
+  mk_production : N → clause Σ N → production Σ N.
+
+Arguments mk_production {_} {_}.
+
+Notation "A ↦ α" := (mk_production A α) (at level 40).
+
+Global Instance production_elem_of_grammar Σ N : ElemOf (production Σ N) (grammar Σ N) := λ p G,
+  match p with
+  | mk_production A ε => ε_productions G A
+  | mk_production A (atom a) => atom_productions G A a
+  | mk_production A (unary B φ) => unary_productions G A B = Some φ
+  | mk_production A (binary Bl Br φ) => binary_productions G A Bl Br = Some φ
+  end.
+
+(* So that one can use notation "A ↦ α ∈ G" *)
+
+(* interfaces for a parse tree *)
+
+Class ParseTree (Σ N : Type) (tree : Type → Type → Type) := {
+  root : tree Σ N → N;
+  word : tree Σ N → sentence Σ;
+  (* validity is decidable *)
+  valid : grammar Σ N → tree Σ N → bool;
+  witness G t A w := root t = A ∧ word t = w ∧ valid G t;
 }.
 
-Arguments start {_} {_}.
-Arguments P {_} {_}.
+Notation "✓{ G } t" := (valid G t) (at level 40, format "'✓{' G '}'  t").
 
-Notation "G ⊢ A ↦ α" := (α ∈ P G A) (at level 60).
+Notation "t ▷ A ={ G }=> w" := (witness G t A w) (at level 40).
 
 (* parsing *)
 
@@ -64,7 +110,7 @@ Arguments token_tree {_} {_}.
 Arguments unary_tree {_} {_}.
 Arguments binary_tree {_} {_}.
 
-Definition root {Σ N : Type} (t : tree Σ N) : N :=
+Definition tree_root {Σ N : Type} (t : tree Σ N) : N :=
   match t with
   | ε_tree R => R
   | token_tree R _ => R
@@ -72,84 +118,150 @@ Definition root {Σ N : Type} (t : tree Σ N) : N :=
   | binary_tree R _ _ => R
   end.
 
-Fixpoint sentence_of {Σ N : Type} (t : tree Σ N) : sentence Σ :=
+Fixpoint tree_word {Σ N : Type} (t : tree Σ N) : sentence Σ :=
   match t with
   | ε_tree _ => []
   | token_tree _ tk => [tk]
-  | unary_tree _ t' => sentence_of t'
-  | binary_tree _ t1 t2 => sentence_of t1 ++ sentence_of t2
+  | unary_tree _ t' => tree_word t'
+  | binary_tree _ t1 t2 => tree_word t1 ++ tree_word t2
   end.
 
-Inductive valid {Σ N : Type} (G : grammar Σ N) : tree Σ N → Prop :=
-  | valid_ε A :
-    G ⊢ A ↦ ε →
-    valid G (ε_tree A)
-  | valid_token A a p :
-    G ⊢ A ↦ atom a →
-    valid G (token_tree A (a @ p))
-  | valid_unary A t' φ :
-    G ⊢ A ↦ unary (root t') φ →
-    valid G t' →
-    (let w := sentence_of t' in w ≠ [] → φ w) →
-    valid G (unary_tree A t')
-  | valid_binary A t1 t2 φ :
-    G ⊢ A ↦ binary (root t1) (root t2) φ →
-    valid G t1 →
-    valid G t2 →
-    (let w1 := sentence_of t1 in let w2 := sentence_of t2 in w1 ≠ [] → w2 ≠ [] → φ w1 w2) →
-    valid G (binary_tree A t1 t2)
-  .
+Fixpoint tree_valid {Σ N : Type} (G : grammar Σ N) (t : tree Σ N) : bool :=
+  match t with
+  | ε_tree A => ε_productions G A
+  | token_tree A tk => atom_productions G A (letter tk)
+  | unary_tree A t' =>
+    match unary_productions G A (tree_root t') with
+    | Some φ => tree_valid G t' && φ (tree_word t')
+    | None => false
+    end
+  | binary_tree A t1 t2 =>
+    match binary_productions G A (tree_root t1) (tree_root t2) with
+    | Some φ => tree_valid G t1 && tree_valid G t2 && φ (tree_word t1) (tree_word t2)
+    | None => false
+    end
+  end.
 
-Notation "✓{ G } t" := (valid G t) (at level 40, format "'✓{' G '}'  t").
+Global Instance ParseTree_tree Σ N : ParseTree Σ N tree := {|
+  root := tree_root;
+  word := tree_word;
+  valid := tree_valid;
+|}.
 
-Definition witness {Σ N : Type} (G : grammar Σ N) (t : tree Σ N) (A : N) (w : sentence Σ) :=
-  root t = A ∧ sentence_of t = w ∧ ✓{G} t.
+Lemma Is_true_andb (b1 b2 : bool) :
+  b1 ∧ b2 → b1 && b2.
+Proof.
+  naive_solver.
+Qed.
 
-Notation "t ▷ A ={ G }=> w" := (witness G t A w) (at level 40).
+Lemma valid_ε_tree {Σ N : Type} (G : grammar Σ N) A :
+  A ↦ ε ∈ G →
+  ✓{G} ε_tree A.
+Proof.
+  naive_solver.
+Qed.
+
+Lemma valid_token_tree {Σ N : Type} (G : grammar Σ N) A tk :
+  A ↦ atom (letter tk) ∈ G →
+  ✓{G} token_tree A tk.
+Proof.
+  naive_solver.
+Qed.
+
+Lemma valid_unary_tree {Σ N : Type} (G : grammar Σ N) A φ t :
+  A ↦ unary (root t) φ ∈ G →
+  φ (word t) →
+  ✓{G} t →
+  ✓{G} unary_tree A t.
+Proof.
+  move => HA ? ? /=.
+  rewrite HA. naive_solver.
+Qed.
+
+Lemma valid_binary_tree {Σ N : Type} (G : grammar Σ N) A φ t1 t2 :
+  A ↦ binary (root t1) (root t2) φ ∈ G →
+  φ (word t1) (word t2) →
+  ✓{G} t1 →
+  ✓{G} t2 →
+  ✓{G} binary_tree A t1 t2.
+Proof.
+  move => HA ? ? ? /=.
+  rewrite HA. naive_solver.
+Qed.
+
+Lemma valid_ε_tree_inv {Σ N : Type} (G : grammar Σ N) A :
+  ✓{G} ε_tree A →
+  A ↦ ε ∈ G.
+Proof.
+  naive_solver.
+Qed.
+
+Lemma valid_token_tree_inv {Σ N : Type} (G : grammar Σ N) A tk :
+  ✓{G} token_tree A tk →
+  A ↦ atom (letter tk) ∈ G.
+Proof.
+  naive_solver.
+Qed.
+
+Lemma valid_unary_tree_inv {Σ N : Type} (G : grammar Σ N) A t :
+  ✓{G} unary_tree A t →
+  ∃ φ, A ↦ unary (root t) φ ∈ G ∧ φ (word t) ∧ ✓{G} t.
+Proof.
+  simpl. case_match; naive_solver.
+Qed.
+
+Lemma valid_binary_tree_inv {Σ N : Type} (G : grammar Σ N) A t1 t2 :
+  ✓{G} binary_tree A t1 t2 →
+  ∃ φ, A ↦ binary (root t1) (root t2) φ ∈ G ∧ φ (word t1) (word t2) ∧
+    ✓{G} t1 ∧ ✓{G} t2.
+Proof.
+  simpl. case_match; naive_solver.
+Qed.
 
 (* derivation *)
 
 Definition derive {Σ N : Type} (G : grammar Σ N) (A : N) (w : sentence Σ) : Prop :=
-  ∃ t, t ▷ A ={G}=> w.
+  ∃ (t : tree Σ N), witness G t A w.
 
 Notation "G ⊨ A ⇒ w" := (derive G A w) (at level 65).
 
-(* proof rules for the judgement G ⊨ A ⇒ w *)
-
 Lemma derive_ε {Σ N : Type} (G : grammar Σ N) A :
-  G ⊢ A ↦ ε → G ⊨ A ⇒ [].
+  A ↦ ε ∈ G →
+  G ⊨ A ⇒ [].
 Proof.
   intros. exists (ε_tree A).
-  repeat split. by constructor.
+  repeat split. by apply valid_ε_tree.
 Qed.
 
 Lemma derive_atom {Σ N : Type} (G : grammar Σ N) A a p :
-  G ⊢ A ↦ atom a → G ⊨ A ⇒ [a @ p].
+  A ↦ atom a ∈ G →
+  G ⊨ A ⇒ [a @ p].
 Proof.
   intros. exists (token_tree A (a @ p)).
-  repeat split. by constructor.
+  repeat split. by apply valid_token_tree.
 Qed.
 
-Lemma derive_unary {Σ N : Type} (G : grammar Σ N) A B (φ : unary_predicate Σ) w :
-  G ⊢ A ↦ unary B φ →
+Lemma derive_unary {Σ N : Type} (G : grammar Σ N) A B φ w :
+  A ↦ unary B φ ∈ G →
+  φ w →
   G ⊨ B ⇒ w →
-  (w ≠ [] → φ w) →
   G ⊨ A ⇒ w.
 Proof.
-  intros ? [t [? [? ?]]] ?. exists (unary_tree A t).
-  repeat split => //. econstructor; naive_solver.
+  intros ? ? [t [? [? ?]]]. exists (unary_tree A t).
+  repeat split => //. eapply valid_unary_tree; naive_solver.
 Qed.
 
-Lemma derive_binary {Σ N : Type} (G : grammar Σ N) A B C (φ : binary_predicate Σ) w1 w2 :
-  G ⊢ A ↦ binary B C φ →
-  G ⊨ B ⇒ w1 →
-  G ⊨ C ⇒ w2 →
-  (w1 ≠ [] → w2 ≠ [] → φ w1 w2) →
+Lemma derive_binary {Σ N : Type} (G : grammar Σ N) A Bl Br φ w1 w2 :
+  A ↦ binary Bl Br φ ∈ G →
+  φ w1 w2 →
+  G ⊨ Bl ⇒ w1 →
+  G ⊨ Br ⇒ w2 →
   G ⊨ A ⇒ w1 ++ w2.
 Proof.
-  intros ? [t1 [? [? ?]]] [t2 [? [? ?]]] ?.
+  intros ? ? [t1 [? [? ?]]] [t2 [? [? ?]]].
   exists (binary_tree A t1 t2).
-  repeat split => //. naive_solver. econstructor; naive_solver.
+  repeat split; try naive_solver.
+  eapply valid_binary_tree; naive_solver.
 Qed.
 
 (* nullability *)
@@ -157,11 +269,11 @@ Qed.
 Definition nullable {Σ N : Type} (G : grammar Σ N) (A : N) : bool.
 Admitted.
 
-Lemma nullable_spec {Σ N : Type} (G : grammar Σ N) A :
-  nullable G A = true → G ⊨ A ⇒ [].
+Fact nullable_spec {Σ N : Type} (G : grammar Σ N) A :
+  nullable G A → G ⊨ A ⇒ [].
 Admitted.
 
-Lemma binary_nullable_l {Σ N : Type} (G : grammar Σ N) A B φ E w :
+(* Lemma binary_nullable_l {Σ N : Type} (G : grammar Σ N) A B φ E w :
   G ⊢ A ↦ binary E B φ →
   nullable G E = true →
   G ⊨ B ⇒ w →
@@ -181,7 +293,7 @@ Proof.
   intros. rewrite <- app_nil_r.
   eapply derive_binary; eauto; last naive_solver.
   by apply nullable_spec.
-Qed.
+Qed. *)
 
 (* Lemma nonterm_derive {Σ N : Type} (G : grammar Σ N) A w :
   G ⊨ A ⇒ w → G ⊨ nonterm A ⇒ w.
@@ -227,30 +339,8 @@ Qed. *)
 
 (* standard notion of ambiguity *)
 
-Definition sentence_ambiguous {Σ N : Type} (G : grammar Σ N) (A : N) (w : sentence Σ) : Prop :=
-  ∃ t1 t2 : tree Σ N,
-    (t1 ▷ A ={G}=> w) ∧ (t2 ▷ A ={G}=> w) ∧ t1 ≠ t2.
+Definition derive_amb {Σ N : Type} (G : grammar Σ N) (A : N) (w : sentence Σ) : Prop :=
+  ∃ t1 t2 : tree Σ N, t1 ▷ A ={G}=> w ∧ t2 ▷ A ={G}=> w ∧ t1 ≠ t2.
 
-Definition ambiguous {Σ N : Type} (G : grammar Σ N) :=
-  ∃ w, sentence_ambiguous G (start G) w.
-
-(* acyclic *)
-
-Inductive derive_nonterm {Σ N : Type} : grammar Σ N → N → N → Prop :=
-  | derive_nonterm_refl G A : derive_nonterm G A A
-  | derive_nonterm_unary G A B φ :
-    (* the derivation is not really A =>* B, but constraint omitted *)
-    G ⊢ A ↦ unary B φ → derive_nonterm G A B
-  | derive_nonterm_binary_nullable_l G A E B φ :
-    G ⊢ A ↦ binary E B φ → nullable G E → derive_nonterm G A B
-  | derive_nonterm_binary_nullable_r G A B E φ :
-    G ⊢ A ↦ binary B E φ → nullable G E → derive_nonterm G A B
-  .
-
-Notation "A ⇒{ G } B" := (derive_nonterm G A B) (at level 65).
-
-Class Acyclic {Σ N : Type} (G : grammar Σ N) := {
-  N_lt : relation N;
-  N_lt_wf : wf N_lt;
-  acyclic : ∀ A B, A ⇒{G} B → N_lt B A;
-}.
+Definition amb {Σ N : Type} (G : grammar Σ N) :=
+  ∃ w, derive_amb G (start G) w.
