theories/ambiguity.v
@@ -1,0 +1,174 @@
+From Coq Require Import ssreflect.
+From stdpp Require Import prelude.
+From ambig Require Import grammar reachable.
+
+(* similarity *)
+
+(* assume input trees have same root and word *)
+
+Definition similar {Σ N : Type} (t1 t2 : tree Σ N) : Prop :=
+  match t1, t2 with
+  | ε_tree _, ε_tree _ => True
+  | token_tree R1 tk1, token_tree R2 tk2 => tk1 = tk2
+  | unary_tree R1 t1, unary_tree R2 t2 => root t1 = root t2
+  | binary_tree R1 tA1 tB1, binary_tree R2 tA2 tB2 =>
+    root tA1 = root tA2 ∧ root tB1 = root tB2 ∧ word tA1 = word tA2
+  | _, _ => False
+  end.
+
+Lemma similar_refl Σ N :
+  Reflexive (@similar Σ N).
+Proof.
+  move => t.
+  destruct t => //=.
+Qed.
+
+(* local ambiguity *)
+
+Definition local_amb {Σ N : Type} `{EqDecision N} `{EqDecision (token Σ)}
+  (G : grammar Σ N) A w : Prop :=
+  ∃ H h, reachable G A w H h ∧
+    ∃ t1 t2, t1 ▷ H ={G}=> h ∧ t2 ▷ H ={G}=> h ∧ ¬ (similar t1 t2).
+
+(* first direction : local ambiguous -> derivation ambiguous *)
+
+Lemma local_amb_implies_derive_amb {Σ N} `{EqDecision N} `{EqDecision (token Σ)}
+  (G : grammar Σ N) A w :
+  local_amb G A w → derive_amb G A w.
+Proof.
+  intros [H [h [Hr [t1 [t2 [Ht1 [Ht2 Hnot]]]]]]].
+  eapply reachable_derive_amb; first apply Hr.
+  exists t1, t2. split; first done. split; first done.
+  intros <-. apply Hnot, similar_refl.
+Qed.
+
+(* second direction : derivation ambiguous -> local ambiguous *)
+
+(* diff two trees with same root and sentence *)
+Fixpoint diff {Σ N : Type} `{!EqDecision N} `{!EqDecision (token Σ)}
+  (t1 t2 : tree Σ N) : option (tree Σ N * tree Σ N) :=
+  match t1, t2 with
+  | ε_tree _, ε_tree _ => None
+  | token_tree _ _, token_tree _ _ =>
+    (* tokens must be eq, so no diff *)
+    None
+  | unary_tree _ t1', unary_tree _ t2' =>
+    (* sentences must be eq, so just compare root *)
+    if bool_decide (root t1' = root t2')
+    then diff t1' t2'
+    else Some (t1, t2)
+  | binary_tree _ tl1 tr1, binary_tree _ tl2 tr2 =>
+    if bool_decide (root tl1 = root tl2 ∧ root tr1 = root tr2 ∧ word tl1 = word tl2)
+    then
+      match diff tl1 tl2 with
+      | Some p => Some p
+      | None => diff tr1 tr2
+      end
+    else Some (t1, t2)
+  | _, _ => Some (t1, t2)
+  end.
+
+Lemma diff_None {Σ N : Type} `{EqDecision N} `{EqDecision (token Σ)} (t1 t2 : tree Σ N) :
+  root t1 = root t2 →
+  word t1 = word t2 →
+  t1 = t2 ↔ diff t1 t2 = None.
+Proof.
+  intros. split.
+  - intros <-.
+    induction t1 => //=.
+    + case_bool_decide => //. by apply IHt1.
+    + case_bool_decide => //=.
+      * rewrite IHt1_1 => //. rewrite IHt1_2 => //.
+      * exfalso. naive_solver.
+  - generalize dependent t2.
+    induction t1 => t2.
+    all: destruct t2 => Hr Hw Hdiff //=.
+    1,2: naive_solver.
+    + simpl in Hr; subst.
+      simpl in Hdiff. case_bool_decide => //.
+      erewrite IHt1; eauto.
+    + simpl in Hr; subst.
+      simpl in Hdiff. case_bool_decide => //.
+      case_match => //.
+      erewrite (IHt1_1 t2_1).
+      erewrite (IHt1_2 t2_2).
+      all: eauto; naive_solver.
+Qed.
+
+Lemma diff_Some_inv {Σ N : Type} `{EqDecision N} `{EqDecision (token Σ)} (t1 t2 t1' t2' : tree Σ N) :
+  root t1 = root t2 →
+  word t1 = word t2 →
+  diff t1 t2 = Some (t1', t2') →
+  root t1' = root t2' ∧ word t1' = word t2'.
+Proof.
+  generalize dependent t2.
+  induction t1 => t2.
+  all: destruct t2 => //= -> Hw Hdiff.
+  all: inversion Hdiff; subst; clear Hdiff => //.
+  - case_bool_decide.
+    * eapply IHt1; eauto.
+    * inversion H0; subst; clear H0. done.
+  - case_bool_decide; first case_match.
+    * naive_solver.
+    * destruct H as [? [? ?]]. eapply (IHt1_2 t2_2); eauto.
+      rewrite H2 in Hw. by eapply app_inv_head_iff.
+    * naive_solver.
+Qed.
+
+Lemma diff_result_not_similar {Σ N : Type} `{EqDecision N} `{EqDecision (token Σ)} (t1 t2 t1' t2' : tree Σ N) :
+  diff t1 t2 = Some (t1', t2') → ¬ (similar t1' t2').
+Proof.
+  generalize dependent t2.
+  induction t1 => t2.
+  all: destruct t2 => //= Hdiff.
+  all: inversion Hdiff; subst; clear Hdiff.
+  all: try naive_solver.
+  - case_bool_decide; naive_solver.
+  - case_bool_decide; first case_match; naive_solver.
+Qed.
+
+Lemma diff_result_subtree {Σ N : Type} `{EqDecision N} `{EqDecision (token Σ)} (t1 t2 t1' t2' : tree Σ N) :
+  diff t1 t2 = Some (t1', t2') → subtree t1' t1 ∧ subtree t2' t2.
+Proof.
+  generalize dependent t2.
+  induction t1 => t2.
+  all: destruct t2 => //= Hdiff.
+  all: inversion Hdiff; subst; clear Hdiff.
+  all: try by split; constructor.
+  - case_bool_decide.
+    * edestruct IHt1; eauto. split; by constructor.
+    * inversion H0; subst. split; by constructor.
+  - case_bool_decide; first case_match.
+    * edestruct (IHt1_1 t2_1); eauto; try congruence. split; by constructor.
+    * edestruct (IHt1_2 t2_2); eauto. split; by constructor.
+    * inversion H0; subst. split; by constructor.
+Qed.
+
+Lemma derive_amb_implies_local_amb {Σ N} `{EqDecision N} `{EqDecision (token Σ)}
+  (G : grammar Σ N) A w :
+  derive_amb G A w → local_amb G A w.
+Proof.
+  intros [t1 [t2 [[Hr1 [Hw1 ?]] [[? [? ?]] ?]]]].
+  have [[t1' t2'] Hdiff] : is_Some (diff t1 t2).
+  { apply not_eq_None_Some. intros Hcontra. apply diff_None in Hcontra => //.
+    all: congruence. }
+  have [Hsub1 Hsub2] := (diff_result_subtree _ _ _ _ Hdiff).
+  exists (root t1'), (word t1').
+  split; first by rewrite -Hr1 -Hw1; apply subtree_reachable.
+  exists t1', t2'.
+  have [? ?] : root t1' = root t2' ∧ word t1' = word t2'.
+  { eapply diff_Some_inv; last eauto. all: congruence. }
+  repeat split => //.
+  1,2: eapply subtree_valid; eauto.
+  eapply diff_result_not_similar; eauto.
+Qed.
+
+(* To sum up *)
+
+Theorem derive_amb_iff_local_amb {Σ N} `{EqDecision N} `{EqDecision (token Σ)}
+  (G : grammar Σ N) A w :
+  derive_amb G A w ↔ local_amb G A w.
+Proof.
+  split; [ apply derive_amb_implies_local_amb
+         | apply local_amb_implies_derive_amb ].
+Qed.
