theories/reachable.v
@@ -1,0 +1,304 @@
+From Coq Require Import ssreflect.
+From stdpp Require Import prelude.
+From ambig Require Import grammar.
+
+(* reachability with layout constraints/predicates *)
+
+Inductive reachable {Σ N : Type} (G : grammar Σ N) : N → sentence Σ (* TODO: necessary? *) → N → sentence Σ → Prop :=
+  | reachable_refl S w S' w' :
+    S = S' →
+    w = w' →
+    reachable G S w S' w'
+  | reachable_unary A B w φ H h :
+    A ↦ unary B φ ∈ G →
+    reachable G B w H h →
+    φ w →
+    reachable G A w H h
+  | reachable_left A Bl w1 Br w2 φ H h :
+    A ↦ binary Bl Br φ ∈ G →
+    reachable G Bl w1 H h →
+    G ⊨ Br ⇒ w2 →
+    φ w1 w2 →
+    reachable G A (w1 ++ w2) H h
+  | reachable_right A Bl w1 Br w2 φ H h :
+    A ↦ binary Bl Br φ ∈ G →
+    reachable G Br w2 H h →
+    G ⊨ Bl ⇒ w1 →
+    φ w1 w2 →
+    reachable G A (w1 ++ w2) H h
+  .
+
+(* tree-representation of reachability *)
+
+Inductive sketch (Σ N : Type) : Type :=
+  | hole : N → sentence Σ → sketch Σ N
+  | unary_sketch : N → sketch Σ N → sketch Σ N
+  | left_sketch : N → sketch Σ N → tree Σ N → sketch Σ N
+  | right_sketch : N → tree Σ N → sketch Σ N → sketch Σ N
+  .
+
+Arguments hole {_} {_}.
+Arguments unary_sketch {_} {_}.
+Arguments left_sketch {_} {_}.
+Arguments right_sketch {_} {_}.
+
+Definition sketch_root {Σ N : Type} (s : sketch Σ N) : N :=
+  match s with
+  | hole H _ => H
+  | unary_sketch R _ => R
+  | left_sketch R _ _ => R
+  | right_sketch R _ _ => R
+  end.
+
+Fixpoint sketch_word {Σ N : Type} (s : sketch Σ N) : sentence Σ :=
+  match s with
+  | hole _ h => h
+  | unary_sketch _ s' => sketch_word s'
+  | left_sketch _ s' t' => sketch_word s' ++ word t'
+  | right_sketch _ t' s' => word t' ++ sketch_word s'
+  end.
+
+Fixpoint sketch_valid {Σ N : Type} (G : grammar Σ N) (s : sketch Σ N) : bool :=
+  match s with
+  | hole _ _ => true
+  | unary_sketch A s' =>
+    match unary_productions G A (sketch_root s') with
+    | Some φ => sketch_valid G s' && φ (sketch_word s')
+    | None => false
+    end
+  | left_sketch A s' t' =>
+    match binary_productions G A (sketch_root s') (root t') with
+    | Some φ => sketch_valid G s' && ✓{G} t' && φ (sketch_word s') (word t')
+    | None => false
+    end
+  | right_sketch A t' s' =>
+    match binary_productions G A (root t') (sketch_root s') with
+    | Some φ => ✓{G} t' && sketch_valid G s' && φ (word t') (sketch_word s')
+    | None => false
+    end
+  end.
+
+Global Instance ParseTree_sketch Σ N : ParseTree Σ N sketch := {|
+  root := sketch_root;
+  word := sketch_word;
+  valid := sketch_valid;
+|}.
+
+Lemma valid_unary_sketch {Σ N : Type} (G : grammar Σ N) A φ s :
+  A ↦ unary (root s) φ ∈ G →
+  φ (word s) →
+  ✓{G} s →
+  ✓{G} unary_sketch A s.
+Proof.
+  intros HA ? ?. simpl.
+  rewrite HA. naive_solver.
+Qed.
+
+Lemma valid_left_sketch {Σ N : Type} (G : grammar Σ N) A φ s t :
+  A ↦ binary (root s) (root t) φ ∈ G →
+  φ (word s) (word t) →
+  ✓{G} s →
+  ✓{G} t →
+  ✓{G} left_sketch A s t.
+Proof.
+  intros HA ? ? ?. simpl.
+  rewrite HA. naive_solver.
+Qed.
+
+Lemma valid_right_sketch {Σ N : Type} (G : grammar Σ N) A φ t s :
+  A ↦ binary (root t) (root s) φ ∈ G →
+  φ (word t) (word s) →
+  ✓{G} t →
+  ✓{G} s →
+  ✓{G} right_sketch A t s.
+Proof.
+  intros HA ? ? ?. simpl.
+  rewrite HA. naive_solver.
+Qed.
+
+Lemma valid_unary_sketch_inv {Σ N : Type} (G : grammar Σ N) A s :
+  ✓{G} unary_sketch A s →
+  ∃ φ, A ↦ unary (root s) φ ∈ G ∧ φ (word s) ∧ ✓{G} s.
+Proof.
+  simpl. case_match; naive_solver.
+Qed.
+
+Lemma valid_left_sketch_inv {Σ N : Type} (G : grammar Σ N) A s t :
+  ✓{G} left_sketch A s t →
+  ∃ φ, A ↦ binary (root s) (root t) φ ∈ G ∧ φ (word s) (word t) ∧ ✓{G} s ∧ ✓{G} t.
+Proof.
+  simpl. case_match; naive_solver.
+Qed.
+
+Lemma valid_right_sketch_inv {Σ N : Type} (G : grammar Σ N) A t s :
+  ✓{G} right_sketch A t s →
+  ∃ φ, A ↦ binary (root t) (root s) φ ∈ G ∧ φ (word t) (word s) ∧ ✓{G} t ∧ ✓{G} s.
+Proof.
+  simpl. case_match; naive_solver.
+Qed.
+
+Fixpoint sig {Σ N : Type} (s : sketch Σ N) : N * sentence Σ :=
+  match s with
+  | hole H h => (H, h)
+  | unary_sketch _ s' => sig s'
+  | left_sketch _ s' _ => sig s'
+  | right_sketch _ _ s' => sig s'
+  end.
+
+Lemma reachable_sketch {Σ N : Type} (G : grammar Σ N) S w H h :
+  reachable G S w H h →
+  ∃ (s : sketch Σ N), sig s = (H, h) ∧ s ▷ S ={G}=> w.
+Proof.
+  induction 1.
+  - exists (hole S w).
+    split; first naive_solver.
+    repeat split.
+  - destruct IHreachable as [s' [? [? [? ?]]]].
+    exists (unary_sketch A s') => /=.
+    split; first done.
+    repeat split; try naive_solver.
+    eapply valid_unary_sketch; naive_solver.
+  - destruct IHreachable as [sl [? [? [? ?]]]].
+    destruct H2 as [tr [? [? ?]]].
+    exists (left_sketch A sl tr) => /=.
+    split; first done.
+    repeat split; try naive_solver.
+    eapply valid_left_sketch; naive_solver.
+  - destruct IHreachable as [sr [? [? [? ?]]]].
+    destruct H2 as [tl [? [? ?]]].
+    exists (right_sketch A tl sr) => /=.
+    split; first done.
+    repeat split; first naive_solver.
+    eapply valid_right_sketch; naive_solver.
+Qed.
+
+(* reachable and ambiguity *)
+
+Fixpoint instantiate {Σ N : Type} (s : sketch Σ N) (t : tree Σ N) :=
+  match s with
+  | hole _ _ => t
+  | unary_sketch R s' => unary_tree R (instantiate s' t)
+  | left_sketch R s' t' => binary_tree R (instantiate s' t) t'
+  | right_sketch R t' s' => binary_tree R t' (instantiate s' t)
+  end.
+
+Lemma instantiate_inj {Σ N} (s : sketch Σ N) :
+  Inj eq eq (instantiate s).
+Proof.
+  move => t1 t2.
+  induction s => /=.
+  all: naive_solver.
+Qed.
+
+Lemma instantiate_root {Σ N} (s : sketch Σ N) t :
+  sig s = (root t, word t) →
+  tree_root (instantiate s t) = root s.
+Proof.
+  destruct s => /=.
+  all: by inversion 1.
+Qed.
+
+Lemma instantiate_word {Σ N} (s : sketch Σ N) t :
+  sig s = (root t, word t) →
+  tree_word (instantiate s t) = word s.
+Proof.
+  induction s => /=.
+  all: inversion 1 as [Hs]; subst => //=.
+  all: specialize (IHs Hs); by rewrite IHs.
+Qed.
+
+Lemma instantiate_valid {Σ N : Type} G (s : sketch Σ N) t :
+  sig s = (root t, word t) →
+  ✓{G} s →
+  ✓{G} t →
+  ✓{G} instantiate s t.
+Proof.
+  intros Hsig Hs Ht.
+  induction s.
+  all: inversion Hsig; subst; clear Hsig.
+  - done.
+  - apply valid_unary_sketch_inv in Hs as [φ [Hp [? ?]]].
+    simpl. rewrite instantiate_root ?instantiate_word ?Hp => //.
+    naive_solver.
+  - apply valid_left_sketch_inv in Hs as [φ [Hp [? [? ?]]]].
+    simpl. rewrite instantiate_root ?instantiate_word ?Hp => //.
+    naive_solver.
+  - apply valid_right_sketch_inv in Hs as [φ [Hp [? [? ?]]]].
+    simpl. rewrite instantiate_root ?instantiate_word ?Hp => //.
+    naive_solver.
+Qed.
+
+Lemma reachable_derive_amb {Σ N} (G : grammar Σ N) A w B w' :
+  reachable G A w B w' →
+  derive_amb G B w' →
+  derive_amb G A w.
+Proof.
+  intros Hr Hamb.
+  apply reachable_sketch in Hr as [s [Hsig [? [? Hs]]]].
+  destruct Hamb as [t1 [t2 [[? [? Ht1]] [[? [? Ht2]] Hne]]]].
+  exists (instantiate s t1), (instantiate s t2).
+  repeat split; simpl.
+  all: try by rewrite instantiate_root; congruence.
+  all: try by rewrite instantiate_word; congruence.
+  all: try by apply instantiate_valid; congruence.
+  intros Hcontra. apply instantiate_inj in Hcontra. contradiction.
+Qed.
+
+(* subtree *)
+
+Inductive subtree {Σ N : Type} : tree Σ N → tree Σ N → Prop :=
+  | subtree_refl t : subtree t t
+  | subtree_unary R t t' : 
+    subtree t t' →
+    subtree t (unary_tree R t')
+  | subtree_left R t tl tr :
+    subtree t tl →
+    subtree t (binary_tree R tl tr)
+  | subtree_right R t tl tr :
+    subtree t tr →
+    subtree t (binary_tree R tl tr)
+  .
+
+Lemma subtree_valid {Σ N : Type} (G : grammar Σ N) t t' :
+  subtree t' t →
+  ✓{G} t →
+  ✓{G} t'.
+Proof.
+  induction 1 => Ht; first done.
+  1: apply valid_unary_tree_inv in Ht as [φ [? [? ?]]].
+  2,3: apply valid_binary_tree_inv in Ht as [φ [? [? [? ?]]]].
+  all: naive_solver.
+Qed.
+
+Lemma subtree_reachable {Σ N : Type} (G : grammar Σ N) t t' :
+  subtree t' t →
+  ✓{G} t →
+  reachable G (root t) (word t) (root t') (word t').
+Proof.
+  induction 1 => Ht; first by constructor.
+  1: apply valid_unary_tree_inv in Ht as [φ [? [? ?]]].
+  2,3: apply valid_binary_tree_inv in Ht as [φ [? [? [? ?]]]].
+  - eapply reachable_unary; eauto.
+  - simpl. eapply reachable_left; eauto. by eexists.
+  - simpl. eapply reachable_right; eauto. by eexists.
+Qed.
+
+(* tree inequality *)
+
+Lemma strict_subtree_ne_unary {Σ N : Type} (t : tree Σ N) A :
+  t ≠ unary_tree A t.
+Proof.
+  induction t; naive_solver.
+Qed.
+
+Lemma strict_subtree_ne_binary_left {Σ N : Type} (t t' : tree Σ N) A :
+  t ≠ binary_tree A t t'.
+Proof.
+  induction t; naive_solver.
+Qed.
+
+Lemma strict_subtree_ne_binary_right {Σ N : Type} (t t' : tree Σ N) A :
+  t ≠ binary_tree A t' t.
+Proof.
+  induction t; naive_solver.
+Qed.
